Added a two more interesting multi-packet theorems

examples/bloomfilter/main_theorem.v
@@ -144,3 +144,245 @@ inv Proc1. inv H6.
 eapply process_packet_prop in H2; [ clear Bf1; destruct H2 as [bf2 [Proc2 Bf2]] | eassumption].
 inv Proc2. inv H5. split; trivial.
 Qed.
+
+Fixpoint multi_process (bf : bloomfilter_state) (l :list (Z * port)): bloomfilter_state * list (option (Z * port)) :=
+  match l with 
+     nil => (bf, nil)
+  | h::t => match process' bf h with
+            (bf1, out) => match multi_process bf1 t with
+                           (bf2, out2) => (bf2, out::out2)
+                          end
+            end
+  end.
+
+Lemma multi_process_length: forall l bf bf2 out, multi_process bf l = (bf2, out) -> length out = length l.
+Proof. induction l; simpl; intros. inv H; trivial.
+destruct (process' bf a). remember (multi_process p l) as x; symmetry in Heqx; destruct x. inv H.
+apply IHl in Heqx. simpl; rewrite Heqx; trivial.
+Qed.
+
+Lemma multi_process_app_inv: forall l1 l2 bf bf2 out, multi_process bf (l1++l2) = (bf2, out) -> 
+      exists bf1 out1 out2, multi_process bf l1 = (bf1, out1) /\ multi_process bf1 l2 = (bf2, out2) /\ out=out1++out2.
+Proof.
+  induction l1; simpl; intros.
++ do 3 eexists; split. reflexivity. split; eauto.
++ destruct (process' bf a) as [bf0 out0].
+  specialize (IHl1 l2 bf0).
+  remember ( multi_process bf0 (l1 ++ l2)) as mp; symmetry in Heqmp; destruct mp. inv H.
+  specialize (IHl1 _ _ (eq_refl _)). destruct IHl1 as [bf1 [out1 [out2 [MP1 [MP2 L]]]]]. subst.
+  rewrite MP1. do 3 eexists; split. reflexivity. rewrite MP2. split; eauto.
+Qed.
+
+Lemma multi_process_prop : forall es bf p es' p',
+  process_packets ge custom_metadata_t es p es' p' ->
+  bf_encode es bf ->
+  exists bf',
+    multi_process bf p = (bf', p') /\ bf_encode es' bf'.
+Proof. intros. generalize dependent bf. induction H; simpl; intros.
++ exists bf; split; trivial.
++ eapply process_packet_prop in H. 2: eassumption.
+  destruct H as [bf2 [K1 BF2]]; rewrite K1; clear K1.
+  apply IHprocess_packets in BF2. destruct BF2 as [bf3 [K2 BF3]]. rewrite K2; clear K2.
+  eexists; split. reflexivity. trivial.
+Qed.
+
+Lemma process_packets_app_inv: forall l1 l2 es es2 output,
+     @process_packets _ _ ge custom_metadata_t es (l1++l2) es2 output ->
+      exists es1 output1 output2, output = output1 ++ output2 /\
+     @process_packets _ _ ge custom_metadata_t es l1 es1 output1 /\
+     @process_packets _ _ ge custom_metadata_t es1 l2 es2 output2.
+Proof.
+ intros l1. induction l1; simpl; intros.
++ do 3 eexists. split. 2:{ split. apply process_packets_nil. eassumption. }
+  reflexivity. 
++ inv H. apply IHl1 in H6; clear IHl1. destruct H6 as [es1 [out1 [out2 [X [PP1 PP2]]]]]; subst.
+  do 3 eexists; split.
+  2:{ split. eapply process_packets_cons; eassumption. eassumption. }
+  reflexivity.
+Qed.
+
+Lemma process_packets_app_inv_encode: forall l1 l2 es es2 output bf,
+     @process_packets _ _ ge custom_metadata_t es (l1++l2) es2 output -> bf_encode es bf ->
+      exists es1 output1 output2 bf1 bf2, output = output1 ++ output2 /\
+     @process_packets _ _ ge custom_metadata_t es l1 es1 output1 /\ multi_process bf l1 = (bf1, output1) /\ bf_encode es1 bf1 /\
+     @process_packets _ _ ge custom_metadata_t es1 l2 es2 output2 /\ multi_process bf1 l2 = (bf2, output2) /\ bf_encode es2 bf2.
+Proof. intros. apply process_packets_app_inv in H. destruct H as [es1 [out1 [out2 [Hout [P1 P2]]]]].
+  destruct (multi_process_prop _ _ _ _ _  P1 H0) as [bf1 [PR1 BF1]].
+  destruct (multi_process_prop _ _ _ _ _  P2 BF1) as [bf2 [PR2 BF2]].
+  do 5 eexists; split. apply Hout.
+  split. eassumption.
+  split. eassumption.
+  split. eassumption.
+  split. eassumption.
+  split. eassumption. eassumption.
+Qed.
+
+Lemma process_packets_length: forall l es1 es2 output,
+     @process_packets _ _ ge custom_metadata_t es1 l es2 output ->
+      length output = length l.
+Proof. intros. induction H; simpl. trivial. f_equal; trivial. Qed.
+
+Lemma multi_process_firewall_aux: forall {l bf z bf1 bf' a out2 out1},
+process' (add Z Z.eqb CRC_pad0 CRC_pad1 CRC_pad2 bf z) a = (bf1, out1) ->
+multi_process bf1 l = (bf', out2) ->
+query Z CRC_pad0 CRC_pad1 CRC_pad2 bf' z = true.
+Proof. 
+induction l; simpl; intros.
++ inv H0. destruct a. destruct p; simpl in H.
+  - inv H. rewrite add_comm. apply bf_add_query_true. apply Z.eqb_refl.
+  - destruct (query Z CRC_pad0 CRC_pad1 CRC_pad2
+        (add Z Z.eqb CRC_pad0 CRC_pad1 CRC_pad2 bf z) z0). 
+    * inv H. apply bf_add_query_true. apply Z.eqb_refl.
+    * inv H. apply bf_add_query_true. apply Z.eqb_refl.
++ remember (process' bf1 a) as x; symmetry in Heqx; destruct x as [bf3 out3].
+  remember (multi_process bf3 l) as y; symmetry in Heqy; destruct y as [bf4 out4].
+  inv H0. destruct a0 as [zz q]. destruct q.
+  - simpl in H. rewrite add_comm in H. inv H. eauto.
+  - simpl in H.
+    remember (query Z CRC_pad0 CRC_pad1 CRC_pad2
+        (add Z Z.eqb CRC_pad0 CRC_pad1 CRC_pad2 bf z) zz) as u; symmetry in Hequ; destruct u.
+    * inv H. eauto.
+    * inv H. eauto.
+Qed.
+
+Lemma multi_process_firewall_endpoints z: forall l bf bf' out, 
+multi_process bf ((z, port_int)::l++[(z, port_ext)]) = (bf', out) -> 
+exists m, out = (Some (z, port_ext)::m++[Some (z, port_int)]).
+Proof. induction l; simpl; intros.
++ rewrite bf_add_query_true in H by apply Z.eqb_refl. inv H. exists (@nil(option (Z * port))). reflexivity.
++ remember (process' (add Z Z.eqb CRC_pad0 CRC_pad1 CRC_pad2 bf z) a) as x; symmetry in Heqx; destruct x as [bf1 out1].
+  remember (multi_process bf1 (l ++ [(z, port_ext)])) as y; symmetry in Heqy; destruct y. inv H.
+  apply multi_process_app_inv in Heqy. destruct Heqy as [bf2 [out2 [out3 [MP1 [MP2 X]]]]]. subst l0.
+  simpl in MP2.
+  remember (query Z CRC_pad0 CRC_pad1 CRC_pad2 bf2 z). destruct b.
+  - inv MP2. exists (out1::out2). simpl; trivial.
+  - rewrite (multi_process_firewall_aux Heqx MP1) in Heqb. discriminate.
+Qed.
+
+Lemma multi_process_firewall {l1 l2 l3 bf bf' out z}:
+      multi_process bf (l1++(z, port_int)::l2++[(z, port_ext)]++l3) = (bf', out) -> 
+exists m1 m2 m3, out = m1++(Some (z, port_ext))::m2++[Some (z, port_int)]++m3 /\
+      length m1=length l1 /\ length m2 = length l2 /\ length m3=length l3.
+Proof. intros. destruct (multi_process_app_inv _ _ _ _ _  H) as [bf1 [m1 [out1 [P1 [Ptail1 X]]]]]; subst out; clear H.
+Proof. intros. specialize (multi_process_app_inv ((z, port_int) :: l2 ++ [(z, port_ext)]) l3 bf1 bf' out1). intros.
+simpl in H. simpl in Ptail1. rewrite <- app_assoc in H. specialize (H Ptail1); clear Ptail1.
+destruct H as [bf3 [out2 [out3 [ST [P3 Hout]]]]]; subst out1.
+remember (multi_process (add Z Z.eqb CRC_pad0 CRC_pad1 CRC_pad2 bf1 z) (l2 ++ [(z, port_ext)]) ) as x; symmetry in Heqx; destruct x.
+inv ST.
+specialize (multi_process_firewall_endpoints z l2 bf1). simpl; intros.
+rewrite Heqx in H. destruct (H _ _ (eq_refl _)) as [m2 M2]; clear H.
+inv M2. exists m1, m2, out3. rewrite <- app_assoc. simpl. split. trivial.
+apply multi_process_length in P1. split; trivial.
+apply multi_process_length in P3. split; trivial.
+apply multi_process_length in Heqx. rewrite 2 app_length in Heqx. simpl in Heqx. lia.
+Qed.
+
+Lemma process_packets_firewall {l1 l2 l3 es es' out z bf}:
+      process_packets ge custom_metadata_t es (l1++(z, port_int)::l2++[(z, port_ext)]++l3) es' out -> bf_encode es bf ->
+  exists bf', bf_encode es' bf' /\
+  exists m1 m2 m3, out = m1++(Some (z, port_ext))::m2++[Some (z, port_int)]++m3 /\
+      length m1=length l1 /\ length m2 = length l2 /\ length m3=length l3.
+Proof. intros.
+  destruct (multi_process_prop _ _ _ _ _ H H0) as [bf' [MP BF']]. exists bf'; split; [trivial |].
+  apply (multi_process_firewall MP).
+Qed.
+
+(*
+(*intermediate property, likely to be deleted eventally*)
+Lemma Firewall': forall l1 l2 l3 es es' output bf,
+     @process_packets _ _ ge custom_metadata_t es (l1++packet1'::l2++packet2'::l3) es' output -> bf_encode es bf ->
+     exists out1 out2 out3 act1 act2,
+     output = out1++act1::out2++act2::out3 /\ 
+     length out1 = length l1 /\ length out2 = length l2 /\ length out3 = length l3.
+Proof. intros. 
+  destruct (process_packets_app_inv_encode _ _ _ _ _ _ H H0) as [es1 [out1 [tail1 [bf1 [bftail [Hout [P1 [MP1 [BF1 [Tail1 [MTail1 BFtail1]]]]]]]]]]]; subst.
+  clear H.
+  apply process_packets_length in P1. clear MTail1 MP1. (*for now*)
+  exists out1; rewrite P1. 
+  inv Tail1. 
+  destruct (process_packet_prop _ _ _ _ _ H3 BF1) as [bf2 [PR2 BF2]]. clear H3.
+  destruct (process_packets_app_inv_encode _ _ _ _ _ _ H6 BF2) as [es3 [out2 [tail2 [bf3 [bftail3 [Hout [P2 [MP3 [BF3 [Tail3 [MTail3 BFtail3]]]]]]]]]]]; subst.
+  clear H6.
+  apply process_packets_length in P2. clear MTail3 MP3. (*for now*)
+  exists out2; rewrite P2. 
+  inv Tail3. 
+  destruct (process_packet_prop _ _ _ _ _ H3 BF3) as [bf4 [PR4 BF4]]. clear H3.
+  specialize (process_packets_length _ _ _ _ H6); intros.
+  exists ps'; rewrite H.
+  do 2 eexists. split. reflexivity. split; eauto.
+Qed.
+Require Import VST.zlist.Zlist.
+
+Lemma app_inv {A}: forall (l1 l2 m1 m2:list A), l1++l2 = m1++m2 -> length l1=length m1 -> l1=m1 /\  l2=m2.
+Proof.
+induction l1; simpl; intros.
++ destruct m1; inv H0. split; trivial.
++ destruct m1; inv H0. inv H. destruct (IHl1 _ _ _ H3 H2); subst. split; trivial. 
+Qed.
+
+Lemma multi_process_firewall_nth n m l bf bf' out z (H: (n<m<length l)%nat):
+      multi_process bf l = (bf', out) ->
+      nth_error l n = Some (z, port_int) -> nth_error l m = Some (z, port_ext) ->
+      nth_error l n = Some (z, port_ext) /\ nth_error l m = Some (z, port_int).
+Proof. intros.
+destruct (@multi_process_firewall (firstn n l) (firstn m (skipn (S n) l)) (skipn (S (S (m+n))) l) bf bf' out z)
+  as [m1 [m2 [m3 [M [M1 [M2 M3]]]]]].
++ assert (L: l = (firstn n l ++ (z, port_int) :: (firstn m (skipn (S n) l)) ++ [(z, port_ext)] ++ skipn (S (S (m + n))) l)).
+  { clear H0. apply nth_error_split in H1. destruct H1 as [l1 [l2 [Hl Len1]]].
+    specialize (firstn_skipn n l); intros X. rewrite <- X at 1. f_equal. symmetry in X.
+    assert (Datatypes.length l1 = Datatypes.length (firstn n (l1 ++ (z, port_int) :: l2))).
+    {  rewrite firstn_length, app_length; simpl. rewrite Nat.min_l; trivial. lia. }
+    rewrite Hl in X. destruct (app_inv  _ _ _ _ X H0). clear X.
+    erewrite (skipn_cons (S n)). intros.
+Search app length.
+
+ subst.  Search nth_error app. rewrite <-(firstn_skipn n l) at 1. f_equal.
+    intros L.  rewrite <- L at 1. firstn_skipnSearch firstn app skipn.
+  rewrite <- L; trivial.
+
+
+ Search nth_error. 
+ ++m3 /\
+
+Definition DummyEntry: (Z * port) := (0, port_int).
+
+Lemma multi_process_firewall_nth n m l bf bf' out z (H: (n<m<length l)%nat):
+      multi_process bf l = (bf', out) ->
+      nth n l DummyEntry = (z, port_int) ->
+      nth m l DummyEntry = (z, port_ext) ->
+      nth n l DummyEntry = (z, port_ext) /\ nth m l DummyEntry = (z, port_int).
+Proof. Search nth_error. 
+ ++m3 /\
+      length m1=length l1 /\ length m2 = length l2 /\ length m3=length l3.
+Search length.
+Check nth. 
+multi_process bf (l1++(z, port_int)::l2++[(z, port_ext)]++l3) = (bf', out)
+   X].
+
+Search process_packets.
+ destruct (multi_process_app_inv _ _ _ _ _  H) as [bf1 [m1 [out1 [P1 [Ptail1 X]]]]]; subst out; clear H.
+Proof. intros. specialize (multi_process_app_inv ((z, port_int) :: l2 ++ [(z, port_ext)]) l3 bf1 bf' out1). intros.
+simpl in H. simpl in Ptail1. rewrite <- app_assoc in H. specialize (H Ptail1); clear Ptail1.
+destruct H as [bf3 [out2 [out3 [ST [P3 Hout]]]]]; subst out1.
+remember (multi_process (add Z Z.eqb CRC_pad0 CRC_pad1 CRC_pad2 bf1 z) (l2 ++ [(z, port_ext)]) ) as x; symmetry in Heqx; destruct x.
+inv ST.
+specialize (multi_process_query_endpoints z l2 bf1). simpl; intros.
+rewrite Heqx in H. destruct (H _ _ (eq_refl _)) as [m2 M2]; clear H.
+inv M2. exists m1, m2, out3. rewrite <- app_assoc. simpl. split. trivial.
+apply multi_process_length in P1. split; trivial.
+apply multi_process_length in P3. split; trivial.
+apply multi_process_length in Heqx. rewrite 2 app_length in Heqx. simpl in Heqx. lia.
+Qed.
+
+Require Import VST.zlist.Zlist.
+
+
+Lemma multi_process_query' n m l bf bf' out z (H: n<m):
+      multi_process bf l = (bf', out) ->
+      Znth n l = (z, port_int) ->
+      Znth m l = (z, port_ext) ->
+      Znth n l = (z, port_ext) /\ Znth m l = (z, port_int). ++m3 /\
+      length m1=length l1 /\ length m2 = length l2 /\ length m3=length l3.
+Search Datatypes.length app. split; trivial.
+
+*)
